translator soudness for kinds - Size is preserved - Shape is preserved - Semantics is preserved

SystemFD/Metatheory/Shape.lean
@@ -399,10 +399,31 @@ theorem kind_shape : Γ ⊢ t : A -> A = □ -> Term.IsKind t := by
 intro j1 j2
 apply kind_shape_lemma j1 j2
 
+@[simp]
+abbrev TypeShapeLemmaVarType (Γ : Ctx Term) : (v : JudgmentVariant) -> JudgmentArgs v -> Prop
+| .prf => λ (t, T) => ∀ x, t = #x -> T.isKind -> Term.IsType Γ t
+| .wf => λ () => True
+
+
+theorem type_shape_lemma_var : Judgment v Γ a -> TypeShapeLemmaVarType Γ v a := by
+intro j <;> induction j <;> simp at *; intros
+case _ Γ x τ wf gt _ ki =>
+constructor; simp
+generalize fh : Γ d@x = f at *
+cases f <;> (unfold Frame.get_type at gt; simp at gt)
+all_goals (cases gt)
+unfold Frame.is_kind; simp
+sorry
+unfold Frame.is_datatype; simp
+sorry
+sorry
+sorry
+sorry
+sorry
 
 @[simp]
-abbrev TypeShapeLemmaType (_ : Ctx Term) : (v : JudgmentVariant) -> JudgmentArgs v -> Prop
-| .prf => λ (t, A) => Term.IsKind A -> Term.IsType t
+abbrev TypeShapeLemmaType (Γ : Ctx Term) : (v : JudgmentVariant) -> JudgmentArgs v -> Prop
+| .prf => λ (t, A) => Term.IsKind A -> Term.IsType Γ t
 | .wf => λ () => True
 
 theorem type_shape_lemma : Judgment v Γ a -> TypeShapeLemmaType Γ v a := by
@@ -411,7 +432,9 @@ case _ ih =>
   intro h; replace ih := ih (by constructor)
   exfalso; apply Term.is_kind_disjoint_is_type h ih
 case _ => intro h; cases h
-case _ => intro h; constructor
+case _ wf gt _ =>
+  intro h; constructor;
+  sorry -- apply type_shape_lemma_var (Judgment.var wf gt);
 case _ => intro h; cases h
 case _ j _ ih1 ih2 =>
   intro h; have lem := kind_shape j rfl
@@ -507,6 +530,6 @@ case _ j1 j2 j3 j4 ih1 ih2 ih3 ih4 =>
   replace ih2 := ih2 lem
   exfalso; apply Term.is_kind_disjoint_is_type h ih2
 
-theorem type_shape : Γ ⊢ t : A -> A.IsKind -> t.IsType := by
+theorem type_shape : Γ ⊢ t : A -> A.IsKind -> t.IsType Γ := by
 intro j1 j2
 apply type_shape_lemma j1 j2
